cts: encoding of finite and infinite paths that actually works

CTL/Satisfaction.lean
@@ -3,6 +3,7 @@ import Mathlib.Data.Set.Functor
 import CTL.Basic
 import TS.Basic
 import TS.Path
+import TS.EFin
 
 namespace CTL
 open TS
@@ -14,48 +15,53 @@ variable {s a p : Type}
 
 mutual
   -- s ⊨ Φ
-  def StateSat (ts : @TS s a p) :=
+  def StateSat :=
     fun Φ st => match Φ with
       | StateFormula.top => True
       | ⬝a               => a ∈ ts.label st
-      | ⬝¬Φ              => ¬(StateSat ts Φ st)
-      | Φ₁ ⬝∧ Φ₂         => (StateSat ts Φ₁ st) ∧ (StateSat ts Φ₂ st)
-      | ⬝∃ φ             => ∃ π : PathFragment.From st, PathSat ts π.1.2 φ
-      | ⬝∀ φ             => ∀ π : PathFragment.From st, PathSat ts π.1.2 φ
+      | ⬝¬Φ              => ¬(StateSat Φ st)
+      | Φ₁ ⬝∧ Φ₂         => (StateSat Φ₁ st) ∧ (StateSat Φ₂ st)
+      | ⬝∃ φ             => ∃ π : PathFragment.From ts st, PathSat π.1.2 φ
+      | ⬝∀ φ             => ∀ π : PathFragment.From ts st, PathSat π.1.2 φ
 
   -- π ⊨ φ
-  def PathSat (ts : @TS s a p) (π : ts.PathFragment n) :=
+  def PathSat (π : ts.PathFragment n) :=
     fun
-     | ⬝◯ Φ   => StateSat ts Φ (π.get ⟨1, _⟩)
-     | Φ ⬝U Ψ => ∃ j : FinWithInf n.succ, (∀ k : FinWithInf ↑j, StateSat ts Φ (π.get k)) ∧ (StateSat ts Ψ (π.get j))
+      | ⬝◯ Φ   => StateSat Φ (π.second)
+      | Φ ⬝U Ψ => ∃ j : EFin (Order.succ n), (StateSat Ψ (π.get j)) ∧ ∀ k : EFin j.val, StateSat Φ (π.get (EFin.castLT j.lt k))
 end
 
 -- Sat(Φ)
-def TS.SatState := { st : s // ts.StateSat Φ st }
-def TS.satStateSet := @Set.range s (ts.SatState Φ) Subtype.val
+def SatState := { st : s // StateSat ts Φ st }
+def satStateSet := @Set.range s (SatState ts Φ) Subtype.val
 
 -- TS ⊨ Φ
-def TS.Sat := ∀ st ∈ ts.initial, ts.StateSat Φ st
+def Sat := ∀ st ∈ ts.initial, StateSat ts Φ st
 
-@[simp]
-theorem TS.Sat.subset_iff : (ts.Sat Φ) ↔ (ts.initial ⊆ ts.satStateSet Φ) :=
-  by
-    apply Iff.intro
-    . intro sat st mem
-      exact Set.mem_range_self (⟨st, sat st mem⟩ : ts.SatState Φ)
-    . intro sub st mem
-      specialize sub mem
-      unfold TS.satStateSet at sub
-      rw [Set.mem_range] at sub
-      obtain ⟨stSat, refl⟩ := sub
-      rw [← refl]
-      exact Subtype.property stSat
+namespace Sat
+  @[simp]
+  theorem Sat.subset_iff : (Sat ts Φ) ↔ (ts.initial ⊆ satStateSet ts Φ) :=
+    by
+      apply Iff.intro
+      . intro sat st mem
+        exact Set.mem_range_self (⟨st, sat st mem⟩ : SatState ts Φ)
+      . intro sub st mem
+        specialize sub mem
+        unfold satStateSet at sub
+        rw [Set.mem_range] at sub
+        obtain ⟨stSat, refl⟩ := sub
+        rw [← refl]
+        exact Subtype.property stSat
+end Sat
 
-@[simp]
-theorem TS.StateSat.potentialAll_def : ts.StateSat (⬝∃■Φ) st ↔ ∃π : ts.PathFrom st, ∀j, ts.StateSat Φ (π.1.2.get j) := by
-  simp [StateFormula.potentialAll, TS.StateSat, StateFormula.inevitable, TS.PathSat]
+namespace StateSat
+  @[simp]
+  theorem potentialAll_def {st : s} : StateSat ts (⬝∃■Φ) st ↔ ∃π : PathFragment.From ts st, ∀j, StateSat ts Φ (π.1.2.get j) := by
+    simp [StateFormula.potentialAll, StateSat, StateFormula.inevitable, PathSat]
 
-@[simp]
-theorem TS.StateSat.invariant_def : ts.StateSat (⬝∀■Φ) st ↔ ∀π : ts.PathFrom st, ∀j, ts.StateSat Φ (π.1.2.get j) := by
-  simp [StateFormula.invariant, TS.StateSat, StateFormula.potential, TS.PathSat]
+  @[simp]
+  theorem invariant_def : StateSat ts (⬝∀■Φ) st ↔ ∀π : PathFragment.From ts st, ∀j, StateSat ts Φ (π.1.2.get j) := by
+    simp [StateFormula.invariant, StateSat, StateFormula.potential, PathSat]
+end StateSat
+
 end CTL
