TS/EFin.lean
@@ -1,8 +1,39 @@
 import Mathlib.Data.ENat.Basic
 
 inductive EFin : ℕ∞ → Type where
-  | fin {n m : ℕ} : (lt : n < m) → EFin m
-  | inf (n   : ℕ) : EFin ⊤
+  | fin (i : ℕ) (lt : i < n) : EFin n
+  | inf (i : ℕ) : EFin ⊤
 
 namespace EFin
+@[inline]
+def val : EFin n → ℕ
+  | .fin i _ => i
+  | .inf i   => i
+
+@[inline]
+def lt (i : EFin n) : i.val < n :=
+  match i with
+  | .fin _ lt => WithTop.coe_lt_coe.2 lt
+  | .inf i    => WithTop.coe_lt_top i
+
+attribute [coe] EFin.val
+
+def succ : EFin n → EFin (Order.succ n)
+  | .fin i lt => fin i.succ (Nat.succ_lt_succ lt)
+  | .inf i    => inf i
+
+@[inline]
+def castInfty {n : ℕ} (i : EFin n) : EFin ⊤ :=
+  match i with | .fin i _ => .inf i
+
+@[inline]
+def castLT {m : ℕ} {n : ℕ∞} (h : m < n) (i : EFin m) : EFin n :=
+  match n with
+  | ⊤      => castInfty i
+  | some _ => match i with | .fin i lt => fin i (Nat.lt_trans lt (WithTop.some_lt_some.1 h))
+
+@[inline]
+def castLT' {m n : ℕ} (i : EFin m) (h : i.val < n) : EFin n :=
+  match i with | .fin i _ => (fin i h : EFin n)
+
 end EFin
